src/packager/lief.ml
@@ -6,6 +6,7 @@ let elf: elf typ = ptr void
 let rel_t = funptr (uint64_t @-> returning uint64_t)
 
 let parse = foreign "lief_parse" (string @-> returning elf)
+let parse_mem = foreign "lief_parse_mem" (ptr uint8_t @-> size_t @-> returning elf)
 let get_text = foreign "lief_get_text" (elf @-> ptr size_t @-> ptr uint64_t @-> returning (ptr uint32_t))
 let get_after = foreign "lief_get_after" (elf @-> returning uint64_t)
 let get_entrypoint = foreign "lief_get_entrypoint" (elf @-> returning uint64_t)
