theories/Decode.v
@@ -16,19 +16,19 @@ Variant ityp :=
   | TBZ (b5 op b40 imm Rt: int).
 
 Definition dc_b_cond (n:int) :=
-  let o0 := n`[4] in
-  let o1 := n`[24] in
+  let o0 := n:[4] in
+  let o1 := n:[24] in
   if (o0 =? 0) && (o1 =? 0)
-  then let imm := n`[5,24] in
-       let cond := n`[0,4] in
+  then let imm := n:[5,24] in
+       let cond := n:[0,4] in
        Bcond imm cond
   else ignore.
 Definition dc_b_reg (n:int) :=
-  let opc := n`[21,25] in
-  let op2 := n`[16,21] in
-  let op3 := n`[10,16] in
-  let Rn := n`[5,10] in
-  let op4 := n`[0,5] in
+  let opc := n:[21,25] in
+  let op2 := n:[16,21] in
+  let op3 := n:[10,16] in
+  let Rn := n:[5,10] in
+  let op4 := n:[0,5] in
   if (op2 =? 31) then
     if (opc =? 0) then
       if (op3 =? 0) then
@@ -48,58 +48,58 @@ Definition dc_b_reg (n:int) :=
     else invalid
   else ignore.
 Definition dc_b_imm n :=
-  let imm26 := n`[0,26] in
-  let op := n`[31] in
+  let imm26 := n:[0,26] in
+  let op := n:[31] in
   if (op =? 0)
   then B imm26
   else BL imm26.
 Definition dc_cb n :=
-  let sf := n`[31] in
-  let op := n`[24] in
-  let imm := n`[5,24] in
-  let Rt := n`[0,5] in
+  let sf := n:[31] in
+  let op := n:[24] in
+  let imm := n:[5,24] in
+  let Rt := n:[0,5] in
   CBZ sf op imm Rt.
 Definition dc_tb n :=
-  let b5 := n`[31] in
-  let op := n`[24] in
-  let b40 := n`[19,24] in
-  let imm := n`[5,19] in
-  let Rt := n`[0,5] in
+  let b5 := n:[31] in
+  let op := n:[24] in
+  let b40 := n:[19,24] in
+  let imm := n:[5,19] in
+  let Rt := n:[0,5] in
   TBZ b5 op b40 imm Rt.
 
 Definition dc_b (n:int) :=
-  let op0 := n`[29,32] in
+  let op0 := n:[29,32] in
   if (op0 =? 2) then
-    if (n`[25] =? 0)
+    if (n:[25] =? 0)
     then dc_b_cond n
     else ignore
   else if (op0 =? 6) then
-    if (n`[25] =? 1)
+    if (n:[25] =? 1)
     then dc_b_reg n
     else ignore
   else if (op0 =? 0) || (op0 =? 4) then
     dc_b_imm n
   else if (op0 =? 1) || (op0 =? 5) then
-    if (n`[25] =? 0)
+    if (n:[25] =? 0)
     then dc_cb n
     else dc_tb n
   else ignore.
 Definition dc_pcr n :=
-  let op := n`[31] in
-  let immlo := n`[29,31] in
-  let immhi := n`[5,24] in
-  let Rd := n`[0,5] in
+  let op := n:[31] in
+  let immlo := n:[29,31] in
+  let immhi := n:[5,24] in
+  let Rd := n:[0,5] in
   let imm := immhi << 2 lor immlo in
   if (op =? 0)
   then ADR imm Rd
   else ADRP imm Rd.
 Definition dc_dpi n :=
-  let op0 := n`[23,26] in
+  let op0 := n:[23,26] in
   if (op0 =? 0) || (op0 =? 1)
   then dc_pcr n
   else ignore.
 Definition decode n :=
-  let op0 := n`[25,29] in
+  let op0 := n:[25,29] in
   if (op0 =? 10) || (op0 =? 11)
   then dc_b n
   else if (op0 =? 8) || (op0 =? 9)
